Added L2_5 which I forgot to add before (thanks Abhishek).  In the middle of working in some proofs, so commented out some lines in _CoqProject, but the translation files are still compiled by make.

theories/L2_5_box/wNorm.v
@@ -1,15 +1,19 @@
+(****)
+Add LoadPath "../common" as Common.
+Add LoadPath "../L2_5_box" as L2_5.
+(****)
 
 Require Import Coq.Lists.List.
 Require Import Coq.Strings.String.
 Require Import Coq.Strings.Ascii.
 Require Import Coq.Arith.EqNat.
 Require Import Coq.Arith.Compare_dec.
-Require Import Common.AstCommon.
-Require Import L1g.term.
-Require Import L1g.program.
-Require Import L1g.wndEval.
-Require Import L1g.awndEval.
-Require Import L1g.wcbvEval.
+Require Import Common.Common.
+Require Import L2_5.term.
+Require Import L2_5.program.
+Require Import L2_5.wndEval.
+Require Import L2_5.awndEval.
+Require Import L2_5.wcbvEval.
 
 Local Open Scope string_scope.
 Local Open Scope bool.
@@ -18,16 +22,7 @@ Set Implicit Arguments.
 
 
 (** Weak typed normal form: normal form of wndEval:
-*** no wndEval steps possible (including no step(**********
-Lemma wndEvalRTC_Prf:
-  forall t t', wndEvalRTC t t' -> wndEvalRTC (TProof t) t'.
-induction 1.
-- constructor. constructor.
--  constructor. constructor. apply sPrf. assumption.
-- eapply wERTCtrn. apply IHwndEvalRTC1. apply IHwndEvalRTC2.
-Qed.
- **********)
-s in type fields.
+*** no wndEval steps possible (including no steps in type fields.
 *** TRel is not itself a weak typed normal form, but unbound indices
 *** may occur under a binder in a weak typed normal form
 **)
@@ -35,18 +30,19 @@ Section Sec_environ.
 Variable p: environ Term.
   
 Inductive WNorm: Term -> Prop :=
-| WNLam: forall nm ty bod, WNorm ty -> WNorm (TLambda nm ty bod)
-| WNProd: forall nm ty bod, WNorm ty -> WNorm (TProd nm ty bod)
+| WNPrf: WNorm TProof
+| WNLam: forall nm bod, WNorm (TLambda nm bod)
+| WNProd: forall nm bod, WNorm (TProd nm bod)
 | WNFix: forall ds br, WNorm (TFix ds br)
 | WNAx: WNorm TAx
-| WNCase: forall mch n ty brs,
-            WNorm mch -> WNorm ty -> WNorms brs -> ~ isCanonical mch ->
-            WNorm (TCase n ty mch brs)
+| WNCase: forall mch n brs,
+            WNorm mch -> WNorms brs -> ~ isCanonical mch ->
+            WNorm (TCase n mch brs)
 | WNConstruct: forall i n arty, WNorm (TConstruct i n arty)
 | WNInd: forall i, WNorm (TInd i)
 | WNSort: forall srt, WNorm (TSort srt)
 | WNApp: forall fn t ts,
-           WNorm fn -> WNorms (tcons t ts) ->
+           WNorm fn -> WNorm t -> WNorms ts ->
            ~ isLambda fn -> ~ isFix fn -> ~ isApp fn ->
            WNorm (TApp fn t ts)
 with WNorms: Terms -> Prop :=
@@ -63,38 +59,35 @@ Ltac lft := solve [left; constructor; assumption].
 (*** Is this desirable ??? ***
 Lemma WNorm_WFapp:
   (forall s, WNorm s -> WFapp s) /\
-  (forall ss, WNorms ss -> WFapps ss) /\
-  (forall dts, WDNorms dts -> WFappDs dts).
+  (forall ss, WNorms ss -> WFapps ss).
 Proof.
   apply WNormWNorms_ind; intros; constructor; try assumption.
 Qed.
  ****)
 
+(*****
 (** WNorm is decidable **)
 Lemma WNorm_dec:
   (forall t, WNorm t \/ ~ WNorm t) /\
   (forall ts, WNorms ts \/ ~ WNorms ts) /\
-  (forall (ds:Defs), True).
+  (forall ds:Defs, True).
 Proof.
   apply TrmTrmsDefs_ind; intros; auto;
   try (solve[right; intros h; inversion h]);
   try (solve[left; constructor]).
-  - destruct H; [lft|rght].  
+  - destruct H; [lft|rght].
   - destruct H; [lft|rght].
   - destruct (isLambda_dec t). rght.
     destruct (isFix_dec t). rght.
-    destruct (isApp_dec t). rght.
     destruct H, H0, H1; try rght.
-    + left. apply WNApp; auto. constructor; assumption.
-    + right. intros h; inversion_Clear h. inversion_Clear H6. contradiction.
-    + right. intros h; inversion_Clear h. inversion_Clear H6. contradiction.
-    + right. intros h; inversion_Clear h. inversion_Clear H6. contradiction.
+    + left. apply WNApp; auto.
   - destruct H, H0, H1; try rght.
     + destruct (isCanonical_dec t0); try rght.
       * left. constructor; auto.
   - destruct H, H0; try rght.
     + left. constructor; assumption.
 Qed.
+*****)
 
 Lemma WNorms_tappendl:
   forall ts us, WNorms (tappend ts us) -> WNorms ts.
@@ -106,14 +99,54 @@ Proof.
 Qed.
 
 Lemma tappend_WNorms:
-  forall ts, WNorms ts -> forall us, WNorms us ->
-                                     WNorms (tappend ts us).
+  forall ts, WNorms ts -> forall us, WNorms us -> WNorms (tappend ts us).
 Proof.
-  induction 1; intros; cbn. assumption.
-  constructor; intuition.
+  induction 1; intros.
+  - cbn. assumption.
+  - cbn. constructor; try assumption. apply IHWNorms. assumption.
 Qed.
 
-(********************
+Lemma WNorm_mkApp:
+  (forall fn, WNorm fn -> ~ isLambda fn -> ~ isFix fn -> 
+              forall args, WNorms args -> WNorm (mkApp fn args)).
+Proof.
+  induction 1; intros; destruct args;
+  try (solve[rewrite mkApp_tnil_ident; intuition]);
+  try (solve[rewrite mkApp_goodFn; try not_isApp]);
+  try (solve[inversion_Clear H1; repeat constructor; try assumption;
+             try not_isFix; not_isApp]).
+  - inversion_Clear H4. constructor; try assumption.
+    + constructor; try assumption.
+    + not_isApp.
+  - inversion_Clear H7. constructor; try assumption.
+    + eapply tappend_WNorms; try assumption.  constructor; try assumption.
+Qed.
+
+(*********
+Lemma WNorm_TApp:
+  (forall fn, WNorm fn -> ~ isLambda fn -> ~ isFix fn -> 
+              forall arg, WNorm arg -> forall args, WNorms args ->
+                                                    WNorm (TApp fn arg args)).
+Proof.
+  induction 1; intros;
+  try (solve[destruct H3 as [x0 [x1 [x2 j]]]; discriminate]);
+  try (solve[repeat constructor; try assumption; not_isApp]).
+  - repeat constructor; try assumption.
+    
+  try (elim H; not_isLambda). destruct args;
+  try (solve[rewrite mkApp_tnil_ident; intuition]);
+  try (solve[rewrite mkApp_goodFn; try not_isApp]);
+  try (solve[inversion_Clear H1; repeat constructor; try assumption;
+             try not_isFix; not_isApp]).
+  - inversion_Clear H4. constructor; try assumption.
+    + constructor; try assumption.
+    + not_isApp.
+  - inversion_Clear H7. constructor; try assumption.
+    + eapply tappend_WNorms; try assumption.  constructor; try assumption.
+Qed.
+   try (repeat constructor; intuition).
+
+ (***********)
 Lemma Wcbv_WNorm:
   WFaEnv p ->
   (forall t s, WcbvEval p t s -> WFapp t -> WNorm s) /\
@@ -122,32 +155,37 @@ Proof.
   intros hp.
   apply WcbvEvalEvals_ind; simpl; intros; try (solve[constructor]);
   try inversion_Clear H0; intuition.
-  - apply H. assert (j:= Lookup_pres_WFapp hp l). inversion j. assumption.
+  - apply H. assert (j:= e). unfold lookupDfn in e.
+    destruct (lookup nm p); try discriminate.
+    + destruct e0; try discriminate.
+      myInjection e. eapply lookupDfn_pres_WFapp; eassumption.
   - inversion_Clear H2. apply H1. 
     assert (j:= proj1 (wcbvEval_pres_WFapp hp) _ _ w H7). inversion_Clear j.
-    assert (j: WFapps (tcons a1' args')).
-    { apply (proj2 (wcbvEval_pres_WFapp hp) _ _ w0).
-      constructor; assumption. }
+    assert (j: WFapps (tcons a1' args)).
+    { constructor; try assumption.
+     eapply (proj1 (wcbvEval_pres_WFapp hp)); eassumption. }
     inversion_Clear j.
     apply whBetaStep_pres_WFapp; try assumption.
   - inversion_Clear H1. apply H0. apply instantiate_pres_WFapp.
     + assumption.
     + refine (proj1 (wcbvEval_pres_WFapp hp) _ _ _ _); eassumption.
-  - inversion_clear H2. specialize (H H4). inversion_Clear H.
-    assert (k:= proj1 (wcbvEval_pres_WFapp hp) _ _ w H4). inversion_Clear k.
-    apply H1.
+  - inversion_clear H1. specialize (H H3). inversion_Clear H.
+    assert (k:= proj1 (wcbvEval_pres_WFapp hp) _ _ w H3). inversion_Clear k.
+    apply H0.
     refine (pre_whFixStep_pres_WFapp _ _ _); try eassumption.
-    eapply (dnthBody_pres_WFapp H2 _ e).
-    eapply (proj2 (wcbvEval_pres_WFapp hp)). eassumption.
+    eapply (dnthBody_pres_WFapp H1 _ e).
     constructor; assumption.
-  - inversion_Clear H1. specialize (H H6).
-    assert (j: WFapp fn').
-    { eapply (proj1 (wcbvEval_pres_WFapp hp)); eassumption. }
-    rewrite mkApp_goodFn; try assumption.
-    constructor; try assumption.
-    + admit.
-    +
-      
+  - inversion_Clear H1.
+    assert (j0: WFapps (tcons arg args)). constructor; assumption.
+    specialize (H0 j0). inversion_Clear H0.
+    specialize (H H6). rewrite mkApp_goodFn.
+    + constructor; try eassumption.
+    
+    apply H1.
+    assert (k:= proj1 (wcbvEval_pres_WFapp hp) _ _ w H7).
+    assert (k0:= proj2 (wcbvEval_pres_WFapp hp) _ _ w0 j0).
+    apply mkApp_pres_WFapp; assumption.
+
   - inversion_Clear H2. 
     assert (j0: WFapps (tcons arg args)). constructor; assumption.
     specialize (H0 j0). inversion_Clear H0.
@@ -168,7 +206,7 @@ Proof.
   - inversion H.
   - inversion_Clear H1. constructor; intuition.
 Qed.
-*****************)
+**********************)
 
 (** If a program is in weak normal form, it has no wndEval step **)
 Lemma wNorm_no_wndStep_lem:
@@ -178,10 +216,11 @@ Proof.
   apply wndEvalEvals_ind; intros; intros h;
   try (solve[inversion h]);
   try (solve[inversion h; subst; contradiction]).
-  - inversion h. subst. elim H4. exists nm, ty, bod. reflexivity.
-  - inversion h. subst. elim H6.
+  - inversion h. subst. elim H5. exists nm, bod. reflexivity.
+  - inversion h. subst. elim H4.
     eapply canonicalP_isCanonical. eassumption.
-  - inversion h. subst. elim H5. apply IsFix.
+  - inversion h. subst. elim H6. apply IsFix.
+  - inversion_Clear h. elim H. constructor; assumption.
 Qed.
 
 Lemma wNorm_no_wndStep:
