theories/L2_typeStripped/wNorm.v
@@ -1,7 +1,3 @@
-(******)
-Add LoadPath "../common" as Common.
-Add LoadPath "../L2_typeStripped" as L2.
-(******)
 
 Require Import Coq.Lists.List.
 Require Import Coq.Strings.String.
